vera/VerilogEquivalence.v
@@ -1,4 +1,5 @@
 From vera Require Import Verilog.
+From vera Require Import Variables.
 From vera Require VerilogSemantics.
 Import VerilogSemantics.Sort.
 From vera Require Import VerilogSMT.
@@ -37,21 +38,21 @@ Import FunctorNotation.
 Local Open Scope monad_scope.
 Local Open Scope string.
 
-Definition mk_var_same (var : Verilog.variable) : (SMTLib.term SMTLib.Sort_Bool) := 
+Definition mk_var_same (var : Var.t) : (SMTLib.term SMTLib.Sort_Bool) := 
   SMTLib.Term_Eq (SMTLib.Term_Const (verilog_to_smt_var VerilogLeft var))
                  (SMTLib.Term_Const (verilog_to_smt_var VerilogRight var)).
 
-Equations mk_inputs_same (inputs : list Verilog.variable) : SMTLib.term SMTLib.Sort_Bool := {
+Equations mk_inputs_same (inputs : list Var.t) : SMTLib.term SMTLib.Sort_Bool := {
   | [] => SMTLib.Term_True
   | (var :: vars) => SMTLib.Term_And (mk_var_same var) (mk_inputs_same vars)
 }.
 
-Definition mk_var_distinct (var : Verilog.variable) : SMTLib.term SMTLib.Sort_Bool :=
+Definition mk_var_distinct (var : Var.t) : SMTLib.term SMTLib.Sort_Bool :=
   SMTLib.Term_Not (SMTLib.Term_Eq (SMTLib.Term_Const (verilog_to_smt_var VerilogLeft var))
                                   (SMTLib.Term_Const (verilog_to_smt_var VerilogRight var)))
   .
 
-Equations mk_outputs_distinct (inputs : list Verilog.variable) : SMTLib.term SMTLib.Sort_Bool := {
+Equations mk_outputs_distinct (inputs : list Var.t) : SMTLib.term SMTLib.Sort_Bool := {
   | [] => SMTLib.Term_False
   | (var :: vars) => SMTLib.Term_Or (mk_var_distinct var) (mk_outputs_distinct vars)
 }.
